formal/inference/InferenceTest.thy
@@ -179,18 +179,117 @@ proof-
     by auto
 qed
 
-lemma "merge third_branch 5 6 (heuristics [third_trace, second_trace, first_trace]) (satisfies {third_trace, second_trace, first_trace}) = Some a"
+lemma merge_7_5: "merge_states 7 5 merge_5_6 = merge_7_5"
+  by eval
+
+lemma merge_transitions_merge_7_5: "merge_transitions third_branch merge_7_5 (leaves 5 third_branch) (leaves 4 third_branch) (leaves 5 merge_7_5) (arrives 5 merge_7_5)
+           (arrives 4 merge_7_5) (coin 50 100) 5 (coin 50 50) 4 (heuristics [third_trace, second_trace, first_trace]) = Some h_merge_7_5"
+  apply (rule merge_transitions_heuristic)
+    apply (simp add: coin_50_50_cant_directly_subsume_coin_50_100)
+   apply (simp add: coin_50_100_cant_directly_subsume_coin_50_50)
+  by eval
+
+lemma no_drink_choice: "d \<noteq> d' \<Longrightarrow> \<not>choice (select_initialise d m) (select_initialise d' n)"
+  by (simp add: choice_def)
+
+lemma nondeterministic_pairs_h_merge_7_5: "nondeterministic_pairs h_merge_7_5 = {|
+(5, (5, 5), (coin_general 2, 4), coin_general 2, 5),
+(5, (5, 5), (coin_general 2, 5), coin_general 2, 4)
+|}"
 proof-
+  have union:  "ffUnion ((\<lambda>s. state_nondeterminism s (outgoing_transitions s h_merge_7_5)) |`| Inference.S h_merge_7_5) = {|
+                  (5, (5, 5), (coin_general 2, 4), coin_general 2, 5), (5, (5, 8), (coin_general 2, 4), vend pepsi, 6),
+                  (5, (5, 5), (coin_general 2, 5), coin_general 2, 4), (5, (5, 8), (coin_general 2, 5), vend pepsi, 6), (5, (8, 5), (vend pepsi, 6), coin_general 2, 4),
+                  (5, (8, 5), (vend pepsi, 6), coin_general 2, 5), (1, (1, 4), (coin_general 1, 2), vend coke, 3), (1, (4, 1), (vend coke, 3), coin_general 1, 2),
+                  (0, (1, 5), (select_initialise coke 1, 0), select_initialise pepsi 2, 1), (0, (5, 1), (select_initialise pepsi 2, 1), select_initialise coke 1, 0)
+                |}"
+    by eval
+  show ?thesis
+    apply (rule nondeterministic_pairs)
+     apply (simp add: union)
+    apply (simp add: Abs_ffilter Set.filter_def)
+    apply standard
+     apply clarify
+     apply simp
+     apply (case_tac "ab = select_initialise coke 1")
+      apply (simp add: no_drink_choice)
+    apply (case_tac "ac = select_initialise coke 1")
+      apply (simp add: no_drink_choice)
+    apply (case_tac "ab = vend coke")
+      apply (simp add: choice_def)
+     apply (case_tac "ab = vend pepsi")
+    using choice_def apply auto[1]
+    apply (case_tac "ac = vend coke")
+    using choice_def apply auto[1]
+     apply (case_tac "ac = vend pepsi")
+    using choice_def by auto
+qed
+
+lemma direct_subsumption_merge_1: "directly_subsumes (tm oldEFSM) (tm newEFSM) t1FromOld t2 t1 \<Longrightarrow>
+                                    replace_transition newEFSM u1 newFrom t2NewTo t1 t2 = e \<Longrightarrow>
+                                    merge_transitions oldEFSM newEFSM t1FromOld t2FromOld newFrom t1NewTo t2NewTo t1 u1 t2 u2 modifier = Some e"
+  by (simp add: merge_transitions_def)
+
+lemma merge_transitions_coins: "merge_transitions third_branch h_merge_7_5 (leaves 5 third_branch) (leaves 4 third_branch) (leaves 5 h_merge_7_5) (arrives 4 h_merge_7_5)
+                (arrives 4 h_merge_7_5) (coin_general 2) 5 (coin_general 2) 4 (heuristics [third_trace, second_trace, first_trace]) = Some one_coin"
+  apply (simp add: merge_transitions_def directly_subsumes_self)
+  by eval
+
+lemma nondeterministic_pairs_one_coin: "nondeterministic_pairs one_coin = {||}"
+proof-
+  have union: "ffUnion ((\<lambda>s. state_nondeterminism s (outgoing_transitions s one_coin)) |`| Inference.S one_coin) = {|
+(5, (5, 8), (coin_general 2, 5), vend pepsi, 6), (5, (8, 5), (vend pepsi, 6), coin_general 2, 5), (1, (1, 4), (coin_general 1, 2), vend coke, 3),
+   (1, (4, 1), (vend coke, 3), coin_general 1, 2), (0, (1, 5), (select_initialise coke 1, 0), select_initialise pepsi 2, 1),
+   (0, (5, 1), (select_initialise pepsi 2, 1), select_initialise coke 1, 0)|}"
+    by eval
+  show ?thesis
+    apply (rule nondeterministic_pairs)
+     apply (simp add: union)
+    apply (simp add: Abs_ffilter Set.filter_def)
+    apply standard
+    apply clarify
+    apply simp
+    apply (case_tac "ab = select_initialise coke 1")
+     apply (simp add: no_drink_choice)
+    apply (case_tac "ab = select_initialise pepsi 2")
+     apply (simp add: no_drink_choice)
+    apply (case_tac "ab = vend coke")
+     apply (simp add: choice_def)
+    apply (case_tac "ab = coin_general 2")
+     apply (simp add: choice_def)
+    apply (case_tac "ab = vend pepsi")
+     apply (simp add: choice_def)
+    by (simp add: choice_def)
+qed
+
+lemma third_pass: "merge third_branch 5 6 (heuristics [third_trace, second_trace, first_trace]) (satisfies {third_trace, second_trace, first_trace}) = Some one_coin"
+proof-
+  have arrives_5_merge_5_6: "arrives 5 merge_5_6 = 7"
+    by eval
+  have arrives_4_merge_5_6: "arrives 4 merge_5_6 = 5"
+    by eval
+  have arrives_5_h_merge_7_5: "arrives 5 h_merge_7_5 = arrives 4 h_merge_7_5"
+    by eval
+  have satisfactory: "satisfies {third_trace, second_trace, first_trace} (tm one_coin)"
+    by eval
   show ?thesis
     apply (simp add: merge_def merge_5_6 nondeterministic_pairs_merge_5_6 sorted_list_of_fset_def)
+    apply (simp add: arrives_5_merge_5_6 arrives_4_merge_5_6 merge_7_5 merge_transitions_merge_7_5)
+    apply (simp add: nondeterministic_pairs_h_merge_7_5 sorted_list_of_fset_def)
+    apply (simp add: arrives_5_h_merge_7_5 merge_states_reflexive merge_transitions_coins nondeterministic_pairs_one_coin deterministic_def)
+    by (simp add: satisfactory)
+qed
+
+lemma score_4: "sorted_list_of_fset (score one_coin naive_score) = [(2, 1, 5)]"
+  by eval
 
 lemma "iterative_learn traces naive_score heuristics = (tm final)"
   apply (simp add: iterative_learn_def)
   apply (rule tm_same)
   apply (simp add: traces_alt first_branch score_first_branch)
   apply (simp add: first_pass score_2 add_second_branch second_pass)
-  apply (simp add: add_third_branch score_3)
-
+  apply (simp add: add_third_branch score_3 third_pass)
+  apply (simp add: score_4)
 
 
 
